Better exception representation

src/Core_Erlang_Automated_Exception_Tests.v
@@ -9,13 +9,15 @@ Import Core_Erlang_Functional_Big_Step.Functional_Big_Step.
 
 Import ListNotations.
 
+Definition exception : ValueSequence + Exception := inr (badarith (VTuple [VLit (Integer 5); VTuple []])).
+
 (** 
   Every first example: functional big-step semantics
   Every second example: big-step semantics
 *)
 Example eval_exception_call_fbs :
   (forall (env : Environment) (eff : SideEffectList) (id : nat), 
-  fbs_expr 1000 env id (ECall "+" [^ELit (Integer 5); ^ETuple []]) eff = Result id (inr (badarith (VCons (VLit (Integer 5)) (VTuple [])))) eff).
+  fbs_expr 1000 env id (ECall "+" [^ELit (Integer 5); ^ETuple []]) eff = Result id exception eff).
 Proof.
   intros. simpl. reflexivity.
 Qed.
@@ -24,7 +26,7 @@ Example eval_exception_call :
   forall {env : Environment} {eff : SideEffectList} {id : nat}, 
   |env, id, ECall "+" [^ELit (Integer 5); ^ETuple []], eff|
 -e> 
-  |id, inr (badarith (VCons (VLit (Integer 5)) (VTuple []))), eff|.
+  |id, exception, eff|.
 Proof.
   intros.
   solve.
@@ -50,7 +52,7 @@ Qed.
 Example exception_list_hd_fbs :
   fbs_expr 1000 [] 0 
   (ECons (ECall "+" [^ELit (Integer 5); ^ETuple []]) (ELit (Atom "error"%string))) 
-  [] = Result 0 (inr (badarith (VCons (VLit (Integer 5)) (VTuple [])))) [].
+  [] = Result 0 exception [].
 Proof.
   simpl. reflexivity.
 Qed.
@@ -58,7 +60,7 @@ Qed.
 Example exception_list_hd :
   |[], 0, ECons (ECall "+" [^ELit (Integer 5); ^ETuple []]) (ELit (Atom "error"%string)), []|
 -e>
-  | 0, inr (badarith (VCons (VLit (Integer 5)) (VTuple []))), []|.
+  | 0, exception, []|.
 Proof.
   solve.
 Qed.
@@ -66,7 +68,7 @@ Qed.
 Example exception_list_tl_fbs : 
   fbs_expr 1000 [] 0 (ECons (ELit (Atom "error"%string)) (ECons (ECall "+" [^ELit (Integer 5); ^ETuple []]) (ENil))) []
 =
-  Result 0 (inr (badarith (VCons (VLit (Integer 5)) (VTuple [])))) [].
+  Result 0 exception [].
 Proof.
   simpl. reflexivity.
 Qed.
@@ -74,7 +76,7 @@ Qed.
 Example exception_list_tl : 
   |[], 0, ECons (ELit (Atom "error"%string)) (ECons (ECall "+" [^ELit (Integer 5); ^ETuple []]) (ENil)), []|
 -e> 
-  | 0, inr (badarith (VCons (VLit (Integer 5)) (VTuple []))), []|.
+  | 0, exception, []|.
 Proof.
   solve.
 Qed.
@@ -82,7 +84,7 @@ Qed.
 Example exception_tuple_fbs : 
   fbs_expr 1000 [] 0 (ETuple [^ELit (Atom "error"%string) ; ^ELit (Atom "error"%string); ^ECall "+" [^ELit (Integer 5); ^ETuple []]]) []
 =
-  Result 0 (inr (badarith (VCons (VLit (Integer 5)) (VTuple [])))) [].
+  Result 0 exception [].
 Proof.
   reflexivity.
 Qed.
@@ -90,7 +92,7 @@ Qed.
 Example exception_tuple : 
   |[], 0, ETuple [^ELit (Atom "error"%string) ; ^ELit (Atom "error"%string); ^ECall "+" [^ELit (Integer 5); ^ETuple []]], []|
 -e>
-  | 0, inr (badarith (VCons (VLit (Integer 5)) (VTuple []))), []|.
+  | 0, exception, []|.
 Proof.
   solve.
 Qed.
@@ -157,7 +159,7 @@ Example try_eval_exception_fbs :
                (ECall "+" [^ELit (Integer 5); ^ETuple []]))
   []
 =
-  Result 0 (inr (badarith (VCons (VLit (Integer 5)) (VTuple [])))) []
+  Result 0 exception []
 .
 Proof.
   auto.
@@ -170,7 +172,7 @@ Example try_eval_exception :
                (ECall "+" [^ELit (Integer 5); ^ETuple []]) 
   , []|
 -e>
-  |0, inr (badarith (VCons (VLit (Integer 5)) (VTuple []))), []|
+  |0, exception, []|
 .
 Proof.
   solve.
@@ -184,7 +186,7 @@ Example try_eval_exception2_fbs :
                (ELit (Atom "error"%string)))
   []
 =
-  Result 0 (inr (badarith (VCons (VLit (Integer 5)) (VTuple [])))) []
+  Result 0 exception []
 .
 Proof.
   auto.
@@ -197,7 +199,7 @@ Example try_eval_exception2 :
                (ELit (Atom "error"%string))
   , []|
 -e>
-  | 0, inr (badarith (VCons (VLit (Integer 5)) (VTuple []))), []|
+  | 0, exception, []|
 .
 Proof.
   solve.
@@ -207,7 +209,7 @@ Example eval_case_pat_ex_fbs :
   fbs_expr 1000 [] 0 (ECase (ECall "+" [^ELit (Integer 5); ^ETuple []])
                  [([PVar "X"%string], ^ELit (Atom "true"), ^ELit (Integer 1))]) []
 =
-  Result 0 (inr (badarith (VCons (VLit (Integer 5)) (VTuple [])))) [].
+  Result 0 exception [].
 Proof.
   auto.
 Qed.
@@ -216,7 +218,7 @@ Example eval_case_pat_ex :
   | [], 0, ECase (ECall "+" [^ELit (Integer 5); ^ETuple []])
                  [([PVar "X"%string], ^ELit (Atom "true"), ^ELit (Integer 1))], []|
 -e>
-  | 0, inr (badarith (VCons (VLit (Integer 5)) (VTuple []))), []|.
+  | 0, exception, []|.
 Proof.
   solve.
 Qed.
@@ -262,7 +264,7 @@ Qed.
 Example call_eval_body_ex2_fbs :
   fbs_expr 1000 [] 0 (ECall "+"%string [^ELit (Integer 5); ^ETuple []]) []
 =
-  Result 0 (inr (badarith (VCons (VLit (Integer 5)) (VTuple [])))) [].
+  Result 0 exception [].
 Proof.
   auto.
 Qed.
@@ -270,7 +272,7 @@ Qed.
 Example call_eval_body_ex2 :
   |[], 0, ECall "+"%string [^ELit (Integer 5); ^ETuple []], []|
 -e>
-  | 0, inr (badarith (VCons (VLit (Integer 5)) (VTuple []))), []|.
+  | 0, exception, []|.
 Proof.
   solve.
 Qed.
@@ -278,7 +280,7 @@ Qed.
 Example call_eval_param_ex_fbs :
   fbs_expr 1000 [] 0 (ECall "+"%string [^ELit (Integer 5); ^ECall "+" [^ELit (Integer 5); ^ETuple []]]) []
 =
-  Result 0 (inr (badarith (VCons (VLit (Integer 5)) (VTuple [])))) [].
+  Result 0 exception [].
 Proof.
   auto.
 Qed.
@@ -286,7 +288,7 @@ Qed.
 Example call_eval_param_ex :
   |[], 0, ECall "+"%string [^ELit (Integer 5); ^ECall "+" [^ELit (Integer 5); ^ETuple []]], []|
 -e>
-  |0, inr (badarith (VCons (VLit (Integer 5)) (VTuple []))), []|.
+  |0, exception, []|.
 Proof.
   solve.
 Qed.
@@ -295,7 +297,7 @@ Example let_eval_exception_params_fbs :
   fbs_expr 1000 [] 0 (ELet ["X"%string; "Y"%string] 
                (EValues [ELit (Integer 5); ECall "+" [^ELit (Integer 5); ^ETuple []]]) (ETuple [])) []
 =
-  Result 0 (inr (badarith (VCons (VLit (Integer 5)) (VTuple [])))) [].
+  Result 0 exception [].
 Proof.
   auto.
 Qed.
@@ -304,7 +306,7 @@ Example let_eval_exception_params :
   |[], 0, ELet ["X"%string; "Y"%string] 
                (EValues [ELit (Integer 5); ECall "+" [^ELit (Integer 5); ^ETuple []]]) (ETuple []), []|
 -e>
-  | 0, inr (badarith (VCons (VLit (Integer 5)) (VTuple []))), []|.
+  | 0, exception, []|.
 Proof.
   solve.
 Qed.
@@ -313,7 +315,7 @@ Example let_eval_exception_body_fbs :
   fbs_expr 1000 [] 0 (ELet ["X"%string; "Y"%string] (EValues [ELit (Integer 5); ELit (Integer 5)])
                (ECall "+" [^ELit (Integer 5); ^ETuple []])) []
 =
-  Result 0 (inr (badarith (VCons (VLit (Integer 5)) (VTuple [])))) [].
+  Result 0 exception [].
 Proof.
   auto.
 Qed.
@@ -322,7 +324,7 @@ Example let_eval_exception_body :
   |[], 0, ELet ["X"%string; "Y"%string] (EValues [ELit (Integer 5); ELit (Integer 5)])
                (ECall "+" [^ELit (Integer 5); ^ETuple []]), []|
 -e>
-  |0, inr (badarith (VCons (VLit (Integer 5)) (VTuple []))), []|.
+  |0, exception, []|.
 Proof.
   solve.
 Qed.
@@ -346,7 +348,7 @@ Qed.
 Example apply_eval_exception_closure2_fbs :
   fbs_expr 1000 [] 0 (EApp (ECall "+" [^ELit (Integer 5); ^ETuple []]) [^ELit (Integer 5); ^ELit (Integer 5)]) []
 =
-  Result 0 (inr (badarith (VCons (VLit (Integer 5)) (VTuple [])))) [].
+  Result 0 exception [].
 Proof.
   auto.
 Qed.
@@ -354,7 +356,7 @@ Qed.
 Example apply_eval_exception_closure2 :
   |[], 0, EApp (ECall "+" [^ELit (Integer 5); ^ETuple []]) [^ELit (Integer 5); ^ELit (Integer 5)], []|
 -e>
-  | 0, inr (badarith (VCons (VLit (Integer 5)) (VTuple []))), []|.
+  | 0, exception, []|.
 Proof.
   solve.
 Qed.
@@ -363,7 +365,7 @@ Example apply_eval_exception_param_fbs :
   fbs_expr 1000 [(inl "X"%string, VClos [] [] 0 [] (ELit (Integer 4)))] 1
     (EApp (EVar "X"%string) [^ECall "+" [^ELit (Integer 5); ^ETuple []]]) []
 =
-  Result 1 (inr (badarith (VCons (VLit (Integer 5)) (VTuple [])))) [].
+  Result 1 exception [].
 Proof.
   auto.
 Qed.
@@ -372,7 +374,7 @@ Example apply_eval_exception_param :
   |[(inl "X"%string, VClos [] [] 0 [] (ELit (Integer 4)))], 1,
     EApp (EVar "X"%string) [^ECall "+" [^ELit (Integer 5); ^ETuple []]], []|
 -e>
-  |1, inr (badarith (VCons (VLit (Integer 5)) (VTuple []))), []|.
+  |1, exception, []|.
 Proof.
   solve.
 Qed.
@@ -399,7 +401,7 @@ Example apply_eval_exception_body_fbs :
   fbs_expr 1000 [(inl "X"%string, VClos [] [] 0 [] (ECall "+" [^ELit (Integer 5); ^ETuple []]))] 1
    (EApp (EVar "X"%string) []) []
 =
-  Result 1 (inr (badarith (VCons (VLit (Integer 5)) (VTuple [])))) [].
+  Result 1 exception [].
 Proof.
   auto.
 Qed.
@@ -408,7 +410,7 @@ Example apply_eval_exception_body :
   |[(inl "X"%string, VClos [] [] 0 [] (ECall "+" [^ELit (Integer 5); ^ETuple []]))], 1,
    EApp (EVar "X"%string) [], []|
 -e> 
-  | 1, inr (badarith (VCons (VLit (Integer 5)) (VTuple []))), []|.
+  | 1, exception, []|.
 Proof.
   solve.
 Qed.
@@ -416,7 +418,7 @@ Qed.
 Example letrec_exception_fbs : 
   fbs_expr 1000 [] 0 (ELetRec [(("fun1"%string, 0), ([], ^ELit (Atom "error"%string)))] (ECall "+" [^ELit (Integer 5); ^ETuple []])) []
 =
-  Result 1 (inr (badarith (VCons (VLit (Integer 5)) (VTuple [])))) [].
+  Result 1 exception [].
 Proof.
   auto.
 Qed.
@@ -424,7 +426,7 @@ Qed.
 Example letrec_exception : 
   |[], 0, ELetRec [(("fun1"%string, 0), ([], ^ELit (Atom "error"%string)))] (ECall "+" [^ELit (Integer 5); ^ETuple []]), []|
 -e>
-  |1, inr (badarith (VCons (VLit (Integer 5)) (VTuple []))), []|.
+  |1, exception, []|.
 Proof.
   solve.
 Qed.
@@ -435,7 +437,7 @@ Example map_eval_ex_key_fbs :
                 (^ECall "+" [^ELit (Integer 5); ^ETuple []], ^ELit (Atom "error"%string));
                 (^ELit (Atom "error"%string), ^ELit (Atom "error"%string))]) []
 =
-  Result 0 (inr (badarith (VCons (VLit (Integer 5)) (VTuple [])))) [].
+  Result 0 exception [].
 Proof.
   auto.
 Qed.
@@ -446,7 +448,7 @@ Example map_eval_ex_key :
                 (^ECall "+" [^ELit (Integer 5); ^ETuple []], ^ELit (Atom "error"%string));
                 (^ELit (Atom "error"%string), ^ELit (Atom "error"%string))], []|
 -e>
-  |0, inr (badarith (VCons (VLit (Integer 5)) (VTuple []))), []|.
+  |0, exception, []|.
 Proof.
   solve.
 Qed.
@@ -458,7 +460,7 @@ Example map_eval_ex_val_fbs :
                 (^ELit (Atom "error"%string), ^ELit (Atom "error"%string));
                 (^ELit (Atom "error"%string), ^ELit (Atom "error"%string))]) []
 =
-  Result 0 (inr (badarith (VCons (VLit (Integer 5)) (VTuple [])))) [].
+  Result 0 exception [].
 Proof.
   auto.
 Qed.
@@ -469,7 +471,7 @@ Example map_eval_ex_val :
                 (^ELit (Atom "error"%string), ^ELit (Atom "error"%string));
                 (^ELit (Atom "error"%string), ^ELit (Atom "error"%string))], []|
 -e>
-  |0, inr (badarith (VCons (VLit (Integer 5)) (VTuple []))), []|.
+  |0, exception, []|.
 Proof.
   solve.
 Qed.
@@ -478,7 +480,7 @@ Example seq_eval_ex_1_fbs :
   fbs_expr 1000 [] 0 (ESeq (ECall "+" [^ELit (Integer 5); ^ETuple []])
                 (ELit (Integer 42))) []
 =
-  Result 0 (inr (badarith (VCons (VLit (Integer 5)) (VTuple [])))) [].
+  Result 0 exception [].
 Proof.
   auto.
 Qed.
@@ -488,7 +490,7 @@ Example seq_eval_ex_1 :
                 (ELit (Integer 42))
    , [] |
 -e>
-  | 0, inr (badarith (VCons (VLit (Integer 5)) (VTuple []))), [] |.
+  | 0, exception, [] |.
 Proof.
   solve.
 Qed.
@@ -497,7 +499,7 @@ Example seq_eval_ex_2_fbs :
   fbs_expr 1000 [] 0 (ESeq (ELit (Integer 42))
                 (ECall "+" [^ELit (Integer 5); ^ETuple []])) []
 =
-  Result 0 (inr (badarith (VCons (VLit (Integer 5)) (VTuple [])))) [] .
+  Result 0 exception [] .
 Proof.
   auto.
 Qed.
@@ -507,7 +509,7 @@ Example seq_eval_ex_2 :
                 (ECall "+" [^ELit (Integer 5); ^ETuple []])
    , [] |
 -e>
-  | 0, inr (badarith (VCons (VLit (Integer 5)) (VTuple []))), [] |.
+  | 0, exception, [] |.
 Proof.
   solve.
 Qed.
@@ -536,7 +538,7 @@ Example map_eval_ex_val2_fbs :
                 (^ELit (Atom "error"%string), ^ELit (Atom "error"%string));
                 (^ELit (Atom "error"%string), ^ELit (Atom "error"%string))], ^ECall "+" [^ELit (Integer 5); ^ETuple []])])])])])])]) []
 =
-  Result 0 (inr (badarith (VCons (VLit (Integer 5)) (VTuple [])))) [].
+  Result 0 exception [].
 Proof.
   auto.
 Qed.
@@ -566,7 +568,7 @@ Example map_eval_ex_val2 :
                 (^ELit (Atom "error"%string), ^ELit (Atom "error"%string));
                 (^ELit (Atom "error"%string), ^ELit (Atom "error"%string))], ^ECall "+" [^ELit (Integer 5); ^ETuple []])])])])])])], []|
 -e>
-  |0, inr (badarith (VCons (VLit (Integer 5)) (VTuple []))), []|.
+  |0, exception, []|.
 Proof.
   solve.
 Qed.
